improve lazy rand module

theories/coneris/examples/lazy_rand/lazy_rand_impl.v
@@ -1,5 +1,5 @@
 From iris.algebra Require Import gmap.
-From clutch.coneris Require Import coneris abstract_tape hocap_rand_alt lock lazy_rand_interface.
+From clutch.coneris Require Import coneris hocap_rand_alt lock lazy_rand_interface.
 
 Set Default Proof Using "Type*".
 
@@ -39,7 +39,7 @@ Section impl.
               Hv: !ghost_mapG Σ () (option (nat*nat)),
                 lo:lock, Hl: lockG Σ,
                     (* Hv: !inG Σ (excl_authR (optionO (prodO natO natO))), *)
-                      Ht: !abstract_tapesGS Σ,
+                      (* Ht: !abstract_tapesGS Σ, *)
                         Hr: !rand_spec' val_size
     }.
 
@@ -72,14 +72,14 @@ Section impl.
         
               
   Definition rand_tape_frag α n γ :=
-    (rand_tapes α (option_to_list n) γ.1 ∗ α ◯↪N ( val_size ; option_to_list n ) @ γ.2)%I.
+    (rand_tapes α (option_to_list n) γ )%I.
   
-  Definition rand_tape_auth m γ :=(([∗ set] α∈ dom m, rand_token α γ.1) ∗
-                                   ● ((λ x, (val_size, option_to_list x))<$>m) @ γ.2)%I.
+  (* Definition rand_tape_auth m γ :=(([∗ set] α∈ dom m, rand_token α γ.1) ∗ *)
+  (*                                  ● ((λ x, (val_size, option_to_list x))<$>m) @ γ.2)%I. *)
   
 
   Definition abstract_lazy_rand_inv N γ_tape:=
-    (inv (N.@"tape") (∃ m, rand_tape_auth m γ_tape) ∗ is_rand (N.@"rand") γ_tape.1)%I.
+    ( is_rand (N) γ_tape)%I.
 
 
   Definition option_to_gmap n : gmap () (option (nat*nat)):=
@@ -116,47 +116,43 @@ Section impl.
       abstract_lazy_rand_inv N γ_tape ∗
       is_lock (L:=Hl) γ_lock lk (∃ res, P res ∗ rand_auth res γ_view ∗ l↦(option_to_val res)))%I.
 
-  Lemma rand_tape_presample_impl N c P {HP:∀ n, Timeless (P n)} γ γ_view γ_lock E m α ε (ε2:fin (S val_size) -> R):
-    ↑(N.@"rand")⊆E ->
+  Lemma rand_tape_presample_impl N c P {HP:∀ n, Timeless (P n)} γ γ_view γ_lock E α ε (ε2:fin (S val_size) -> R):
+    ↑(N)⊆E ->
     (∀ x, (0 <= ε2 x)%R)->
     (SeriesC (λ n : fin (S val_size), 1 / S val_size * ε2 n) <= ε)%R ->
     lazy_rand_inv N c P γ γ_view γ_lock -∗
-    rand_tape_auth m γ -∗ rand_tape_frag α None γ -∗ ↯ ε -∗
+     rand_tape_frag α None γ -∗ ↯ ε -∗
     state_update E E (∃ n, 
           ↯ (ε2 n) ∗
-          rand_tape_auth (<[α:=Some (fin_to_nat n)]>m) γ ∗
           rand_tape_frag α (Some (fin_to_nat n)) γ).
   Proof. 
-    iIntros (???) "(%&%&->&#[? Hinv]&#?) [Htokens Htauth] [Htape Hfrag] Herr".
-    iDestruct (abstract_tapes_agree with "[$][$]") as "%H'".
-    rewrite lookup_fmap in H'. apply fmap_Some_1 in H'.
-    destruct H' as (?&Hsome&?). simplify_eq.
+    iIntros (???) "(%&%&->&# Hinv&#?) Htape Herr".
+    (* iDestruct (abstract_tapes_agree with "[$][$]") as "%H'". *)
+    (* rewrite lookup_fmap in H'. apply fmap_Some_1 in H'. *)
+    (* destruct H' as (?&Hsome&?). simplify_eq. *)
     iMod (rand_tapes_presample with "[$][$][$]") as "(%&Htape&?)"; try done.
-    iMod (abstract_tapes_presample with "[$][$]") as "[? H]".
-    iFrame. iModIntro.
-    iSplitL "Htokens".
-    - by rewrite dom_insert_lookup_L.
-    - by rewrite fmap_insert.
+    (* iMod (abstract_tapes_presample with "[$][$]") as "[? H]". *)
+    by iFrame. 
   Qed.
 
-  Lemma lazy_rand_presample_impl N c P {HP: ∀ n, Timeless (P n)} γ γ_view γ_lock Q
-    E  :
-  ↑(N.@"tape") ⊆ E ->
-  lazy_rand_inv N c P γ γ_view γ_lock -∗
-  (∀ m,  rand_tape_auth m γ -∗
-         state_update (E∖↑(N.@"tape")) (E∖↑(N.@"tape"))
-           (∃ m', rand_tape_auth m' γ ∗ Q m m')
-    ) -∗
-    state_update E E (
-        ∃ m m', Q m m'
-      ).
-  Proof.
-    iIntros (?) "(%&%&->&#[Hinv ?]&#?) Hvs".
-    iInv "Hinv" as ">(%&?)" "Hclose".
-    iMod ("Hvs" with "[$]") as "(%&?&?)".
-    iMod ("Hclose" with "[$]") as "_".
-    by iFrame.
-  Qed.
+  (* Lemma lazy_rand_presample_impl N c P {HP: ∀ n, Timeless (P n)} γ γ_view γ_lock Q *)
+  (*   E  : *)
+  (* ↑(N.@"tape") ⊆ E -> *)
+  (* lazy_rand_inv N c P γ γ_view γ_lock -∗ *)
+  (* (∀ m,  rand_tape_auth m γ -∗ *)
+  (*        state_update (E∖↑(N.@"tape")) (E∖↑(N.@"tape")) *)
+  (*          (∃ m', rand_tape_auth m' γ ∗ Q m m') *)
+  (*   ) -∗ *)
+  (*   state_update E E ( *)
+  (*       ∃ m m', Q m m' *)
+  (*     ). *)
+  (* Proof. *)
+  (*   iIntros (?) "(%&%&->&#[Hinv ?]&#?) Hvs". *)
+  (*   iInv "Hinv" as ">(%&?)" "Hclose". *)
+  (*   iMod ("Hvs" with "[$]") as "(%&?&?)". *)
+  (*   iMod ("Hclose" with "[$]") as "_". *)
+  (*   by iFrame. *)
+  (* Qed. *)
 
   Lemma lazy_rand_init_impl N P {HP: ∀ n, Timeless (P n)} :
     {{{ P None }}}
@@ -181,93 +177,78 @@ Section impl.
     iIntros (??) "#Hlock".
     wp_pures.
     iMod (rand_inv_create_spec) as "(%&#Hrand)"; last first.
-    - iMod (abstract_tapes_alloc ∅) as "(%&Hm&_)".
-      iMod (inv_alloc _ _ (∃ m, rand_tape_auth m (_,_)) with "[Hm]") as "#Hinv".
-      { iNext. iExists ∅. rewrite /rand_tape_auth. rewrite fmap_empty.
-        iFrame. by rewrite dom_empty_L. }
+    - (* iMod (abstract_tapes_alloc ∅) as "(%&Hm&_)". *)
+      (* iMod (inv_alloc _ _ (∃ m, rand_tape_auth m (_,_)) with "[Hm]") as "#Hinv". *)
+      (* { iNext. iExists ∅. rewrite /rand_tape_auth. rewrite fmap_empty. *)
+      (*   iFrame. by rewrite dom_empty_L. } *)
       iApply "HΦ". iFrame "Hlock".
-      rewrite /abstract_lazy_rand_inv. iExists (_,_).
-      by iFrame "Hrand Hinv".
+      rewrite /abstract_lazy_rand_inv. iExists _. 
+      by iFrame "Hrand".
     - done.
   Qed.
 
-  Lemma lazy_rand_alloc_tape_impl N c P {HP: ∀ n, Timeless (P n)} γ_tape γ_view γ_lock Q:
-  {{{ lazy_rand_inv N c P γ_tape γ_view γ_lock ∗
-      (∀ (m:gmap val (option nat)) α, ⌜α∉dom m⌝ -∗ |={⊤∖↑N.@"tape"}=> Q α)
+  Lemma lazy_rand_alloc_tape_impl N c P {HP: ∀ n, Timeless (P n)} γ_tape γ_view γ_lock :
+  {{{ lazy_rand_inv N c P γ_tape γ_view γ_lock 
   }}}
       allocate_tape_prog #()
-      {{{ (α: val), RET α; rand_tape_frag α None γ_tape ∗ Q α }}}.
+      {{{ (α: val), RET α; rand_tape_frag α None γ_tape  }}}.
   Proof.
-    iIntros (Φ) "[(%&%&->&#[Hinv ?]&_) Hvs] HΦ".
+    iIntros (Φ) "(%&%&->&#Hinv &_) HΦ".
     rewrite /allocate_tape_prog.
     wp_pures.
     iApply pgl_wp_fupd.
     wp_apply (rand_allocate_tape_spec with "[//]") as (α) "[Htoken Hrand]"; first done.
-    iInv "Hinv" as ">(%m&Htokens&Hauth)" "Hclose".
-    iAssert (⌜α∉dom m⌝)%I as "%".
-    { iIntros "%H".
-      rewrite big_sepS_elem_of_acc; last done.
-      iDestruct "Htokens" as "[? ?]".
-      iApply (rand_token_exclusive with "[$][$]").
-    }
-    iMod ("Hvs" with "[//]") as "HQ".
-    iMod (abstract_tapes_new with "[$]") as "[Hauth Htape]"; last first.
-    - iMod ("Hclose" with "[Hauth Htoken Htokens]").
-      + iExists (<[_:=_]> _). rewrite /rand_tape_auth.  rewrite fmap_insert. iFrame.
-        rewrite dom_insert_L big_sepS_insert; last done.
-        iFrame.
-      + iApply "HΦ". by iFrame.
-    - rewrite lookup_fmap. apply not_elem_of_dom_1 in H. by rewrite H.
+    iApply "HΦ".
+    by iFrame.
   Qed.
 
   Lemma lazy_rand_spec_impl N c P {HP: ∀ n, Timeless (P n)} γ_tape γ_view γ_lock Q1 Q2 α (tid:nat):
   {{{ lazy_rand_inv N c P γ_tape γ_view γ_lock ∗
-      ( ∀ n m, P n -∗ rand_auth n γ_view -∗ rand_tape_auth m γ_tape -∗ state_update (⊤∖↑N.@"tape") (⊤∖↑N.@"tape")
+      ( ∀ n, P n -∗ rand_auth n γ_view -∗ state_update (⊤) (⊤)
              match n with
-             | Some (res, tid') => P n ∗ rand_auth n γ_view ∗ rand_tape_auth m γ_tape ∗ Q1 res tid'
-             | None => ∃ n', rand_tape_frag α (Some n') γ_tape ∗ rand_tape_auth (<[α:=Some n']> m) γ_tape ∗
+             | Some (res, tid') => P n ∗ rand_auth n γ_view ∗ Q1 res tid'
+             | None => ∃ n', rand_tape_frag α (Some n') γ_tape ∗
                               (rand_tape_frag α None γ_tape
-                                      ={⊤∖↑N.@"tape"}=∗  P (Some (n', tid)) ∗ rand_auth (Some (n', tid)) γ_view ∗ Q2 n' tid)
+                                      ={⊤}=∗  P (Some (n', tid)) ∗ rand_auth (Some (n', tid)) γ_view ∗ Q2 n' tid)
              end                                        
       )
   }}}
-      lazy_read_rand_prog c α #tid
+      lazy_read_rand_prog c α #tid 
       {{{ (res' tid':nat), RET (#res', #tid')%V;  (Q1 res' tid' ∨
                                                    Q2 res' tid'
                                 )
       }}}.
   Proof.
-    iIntros (Φ) "[(%&%&->&#[Hinv ?]&#Hlock) Hvs] HΦ".
+    iIntros (Φ) "[(%&%&->&#Hinv&#Hlock) Hvs] HΦ".
     rewrite /lazy_read_rand_prog. wp_pures.
     wp_apply (acquire_spec with "[$]") as "[Hl (%res&HP&(Hauth & Hfrag & %Hvalid)&Hloc)]".
     wp_pures.
     wp_load.
     iApply state_update_pgl_wp.
-    iInv ("Hinv") as ">(%&Htokens&Htauth)" "Hclose".
-    iMod ("Hvs" with "[$][$Hauth $Hfrag//][$]") as "Hcont".
+    (* iInv ("Hinv") as ">(%&Htokens&Htauth)" "Hclose". *)
+    iMod ("Hvs" with "[$][$Hauth $Hfrag//]") as "Hcont".
     destruct res as [[]|].
-    - iDestruct "Hcont" as "(HP&Hauth &Htauth&HQ)".
-      iMod ("Hclose" with "[$Htauth]") as "_".
+    - iDestruct "Hcont" as "(HP&Hauth &HQ)".
       iModIntro. wp_pures.
       wp_apply (release_spec with "[$Hlock $Hl $HP $Hloc $Hauth]").
       iIntros. wp_pures.
       iApply "HΦ". by iFrame.
-    - iDestruct "Hcont" as "(%&[Ht Htfrag] &[Htokens Htauth] & Hvs)".
-      iMod ("Hclose" with "[$Htauth $Htokens]") as "_".
+    - iDestruct "Hcont" as "(%&Ht  & Hvs)".
+      (* iMod ("Hclose" with "[$Htauth $Htokens]") as "_". *)
       iModIntro. wp_pures.
       wp_apply (rand_tape_spec_some with "[$]") as "Htape"; first done.
       iApply fupd_pgl_wp.
-      iInv ("Hinv") as ">(%&Htokens&Htauth)" "Hclose".
-      iDestruct (abstract_tapes_agree with "[$][$]") as "%Hsome".
-      apply lookup_fmap_Some in Hsome.
-      destruct Hsome as ([x|]&?&Hsome); simplify_eq.
-      iMod (abstract_tapes_pop with "[$][$]") as "[Hauth Htape']".
+      (* iInv ("Hinv") as ">(%&Htokens&Htauth)" "Hclose". *)
+      (* iDestruct (abstract_tapes_agree with "[$][$]") as "%Hsome". *)
+      (* apply lookup_fmap_Some in Hsome. *)
+      (* destruct Hsome as ([x|]&?&Hsome); simplify_eq. *)
+      (* iMod (abstract_tapes_pop with "[$][$]") as "[Hauth Htape']". *)
       iMod ("Hvs" with "[$]") as "(HP&Hrand&HQ)".
-      iMod ("Hclose" with "[Hauth Htokens]") as "_".
-      { iExists (<[_:=None]>_).
-        rewrite /rand_tape_auth. rewrite fmap_insert.
-        rewrite dom_insert_lookup_L; last done. iFrame.
-      }
+      (* iMod ("Hclose" with "[Hauth Htokens]") as "_". *)
+      (* { iExists (<[_:=None]>_). *)
+      (*   rewrite /rand_tape_auth. rewrite fmap_insert. *)
+      (*   rewrite dom_insert_lookup_L; last done. iFrame. *)
+      (* } *)
       iModIntro.
       wp_pures.
       wp_store.
@@ -282,12 +263,12 @@ Section impl.
       allocate_tape := allocate_tape_prog;
       lazy_read_rand := lazy_read_rand_prog;
       lazy_rand_interface.rand_tape_frag := rand_tape_frag;
-      lazy_rand_interface.rand_tape_auth := rand_tape_auth;
+      (* lazy_rand_interface.rand_tape_auth := rand_tape_auth; *)
       lazy_rand_interface.rand_auth := rand_auth;
       lazy_rand_interface.rand_frag := rand_frag;
       rand_inv:=lazy_rand_inv;
       rand_tape_presample:=rand_tape_presample_impl;
-      lazy_rand_presample:=lazy_rand_presample_impl;
+      (* lazy_rand_presample:=lazy_rand_presample_impl; *)
       lazy_rand_init:=lazy_rand_init_impl;
       lazy_rand_alloc_tape:=lazy_rand_alloc_tape_impl;
       lazy_rand_spec:=lazy_rand_spec_impl
@@ -298,22 +279,22 @@ Section impl.
   Qed.
   Next Obligation.
     rewrite /rand_tape_frag/=.
-    iIntros (???) "[??]".
+    iIntros (???) "?".
     iDestruct (rand_tapes_valid with "[$]") as "%H".
     by rewrite Forall_singleton in H.
   Qed.
   Next Obligation.
     rewrite /rand_tape_frag.
-    iIntros (????) "[??][??]".
+    iIntros (????) "??".
     iApply (rand_tapes_exclusive with "[$][$]").
   Qed.
-  Next Obligation.
-    rewrite /rand_tape_auth/rand_tape_frag.
-    iIntros (?? x ?) "[??][??]".
-    iDestruct (abstract_tapes_agree with "[$][$]") as "%Hsome".
-    apply lookup_fmap_Some in Hsome.
-    by destruct Hsome as ([[]|]&?&Hsome); destruct x; simplify_eq.
-  Qed.
+  (* Next Obligation. *)
+  (*   rewrite /rand_tape_auth/rand_tape_frag. *)
+  (*   iIntros (?? x ?) "[??][??]". *)
+  (*   iDestruct (abstract_tapes_agree with "[$][$]") as "%Hsome". *)
+  (*   apply lookup_fmap_Some in Hsome. *)
+  (*   by destruct Hsome as ([[]|]&?&Hsome); destruct x; simplify_eq. *)
+  (* Qed. *)
   Next Obligation.
     rewrite /rand_auth.
     iIntros (???) "[??][??]".
@@ -354,4 +335,5 @@ Section impl.
     iFrame.
     by iMod (ghost_map_elem_persist with "[$]") as "$".
   Qed.
+  
 End impl.
